driver/IdSimDemoSpec.v
@@ -1,0 +1,317 @@
+Require Import Sem SimProg Skeleton Mod ModSem SimMod SimModSem SimSymb SimMem Sound SimSymb.
+Require Import Cop Ctypes ClightC.
+Require SimMemId SimMemExt SimMemInj.
+Require SoundTop UnreachC.
+Require SimSymbId SimSymbDrop.
+Require Import DemoSource DemoSpec DemoProof.
+Require Import CoqlibC.
+Require Import ValuesC.
+Require Import LinkingC.
+Require Import MapsC.
+Require Import AxiomsC.
+Require Import Ord.
+Require Import MemoryC.
+Require Import SmallstepC.
+Require Import Events.
+Require Import Preservation.
+Require Import Integers.
+Require Import LocationsC Conventions.
+
+Require Import MatchSimModSem.
+Require Import ClightStepInj ClightStepExt.
+Require Import IdSimExtra IdSimClightExtra.
+Require Import CtypingC.
+Require Import CopC.
+Require Import sflib.
+
+Set Implicit Arguments.
+
+Local Opaque Z.mul Z.add Z.sub Z.div.
+
+Inductive match_states_ext_demo (sm_arg: SimMemExt.t')
+  : unit -> state -> state -> SimMemExt.t' -> Prop :=
+| match_ext
+    i m_src m_tgt sm0
+    (MWFSRC: m_src = sm0.(SimMemExt.src))
+    (MWFTGT: m_tgt = sm0.(SimMemExt.tgt))
+    (MWF: Mem.extends m_src m_tgt)
+  :
+    match_states_ext_demo
+      sm_arg tt
+      (mkstate i m_src)
+      (mkstate i m_tgt)
+      sm0
+.
+
+Section DEMOSOUNDSTATE.
+
+  Variable skenv_link: SkEnv.t.
+  Variable su: Sound.t.
+
+  Inductive sound_state_demo
+    : state -> Prop :=
+  | sound_state
+      i m
+      (WF: Sound.wf su)
+      (MEM: UnreachC.mem' su m)
+      (VALS: Sound.val su (Vlong i))
+      (SKE: su.(Unreach.ge_nb) = skenv_link.(Genv.genv_next))
+    :
+      sound_state_demo (mkstate i m).
+
+End DEMOSOUNDSTATE.
+
+Section DEMOSOUND.
+
+  Variable skenv_link: SkEnv.t.
+
+  Lemma demo_unreach_local_preservation
+    :
+      exists sound_state, <<PRSV: local_preservation (modsem skenv_link tt) sound_state>>
+  .
+  Proof.
+    esplits.
+    eapply local_preservation_strong_horizontal_spec with (sound_state := sound_state_demo skenv_link); eauto.
+    econs; ss; i.
+    - inv INIT. ss. inv SUARG. des. esplits.
+      + refl.
+      + destruct st_init.
+        econs; eauto; ss; inv SKENV; ss.
+      + instantiate (1:=get_mem). ss. rewrite M. refl.
+    - exists su0. esplits; eauto.
+      + refl.
+      + inv SUST. inv FINAL. ss. econs; eauto. ss. clarify.
+      + inv SUST. inv FINAL. ss. refl.
+  Qed.
+
+End DEMOSOUND.
+
+Inductive match_states_demo_internal:
+  state -> state -> meminj -> mem -> mem -> Prop :=
+| match_inj_internal
+    i j m_src m_tgt
+  :
+    match_states_demo_internal
+      (mkstate i m_src)
+      (mkstate i m_tgt)
+      j m_src m_tgt
+.
+
+Inductive match_states_demo (sm_arg: SimMemInj.t')
+  : unit -> state -> state -> SimMemInj.t' -> Prop :=
+| match_states_demo_intro
+    st_src st_tgt j m_src m_tgt sm0
+    (MWFSRC: m_src = sm0.(SimMemInj.src))
+    (MWFTGT: m_tgt = sm0.(SimMemInj.tgt))
+    (MWFINJ: j = sm0.(SimMemInj.inj))
+    (MATCHST: match_states_demo_internal st_src st_tgt j m_src m_tgt)
+    (MWF: SimMemInj.wf' sm0)
+  :
+    match_states_demo
+      sm_arg tt st_src st_tgt sm0
+.
+
+Lemma demo_id
+  :
+    exists mp,
+      (<<SIM: @ModPair.sim SimMemId.SimMemId SimMemId.SimSymbId SoundTop.Top mp>>)
+      /\ (<<SRC: mp.(ModPair.src) = (DemoSpec.module)>>)
+      /\ (<<TGT: mp.(ModPair.tgt) = (DemoSpec.module)>>)
+.
+Proof.
+  eexists (ModPair.mk _ _ _); s.
+  esplits; eauto. instantiate (1:=tt).
+  econs; ss; i.
+  rewrite SIMSKENVLINK in *.
+  eapply match_states_sim; ss.
+  - apply unit_ord_wf.
+  - eapply SoundTop.sound_state_local_preservation.
+  - instantiate (1:= fun sm_arg _ st_src st_tgt sm0 =>
+                       (<<EQ: st_src = st_tgt>>) /\
+                       (<<MWF: sm0.(SimMemId.src) = sm0.(SimMemId.tgt)>>) /\
+                       (<<stmwf: st_src.(DemoSpec.get_mem) =
+                                 sm0.(SimMemId.src)>>)).
+    ss.
+    destruct args_src, args_tgt, sm_arg. ii. inv SIMARGS; ss; clarify.
+    clear SAFESRC. dup INITTGT. inv INITTGT. ss.
+    eexists. eexists (SimMemId.mk tgt tgt). esplits; eauto; ss.
+  - ii. destruct args_src, args_tgt, sm_arg. inv SIMARGS; ss; clarify.
+  - ii. ss. des. clarify.
+  - i. ss. des. clarify. esplits; eauto.
+    econs; ss.
+    + inv FINALSRC; ss.
+    + rewrite <- MWF. inv FINALSRC. ss.
+  - right. ii. des. destruct sm0. ss. clarify. esplits; eauto.
+    + i. exploit H; ss.
+      * econs 1.
+      * i. des; clarify.
+    + i. exists tt, st_tgt1.
+      eexists (SimMemId.mk (get_mem st_tgt1) (get_mem st_tgt1)).
+      esplits; eauto.
+      left. econs; eauto; [econs 1|]. symmetry. apply E0_right.
+      Unshelve. ss. eapply bot4.
+Qed.
+
+Lemma demo_ext_unreach
+  :
+    exists mp,
+      (<<SIM: @ModPair.sim SimMemExt.SimMemExt SimMemExt.SimSymbExtends UnreachC.Unreach mp>>)
+      /\ (<<SRC: mp.(ModPair.src) = (DemoSpec.module)>>)
+      /\ (<<TGT: mp.(ModPair.tgt) = (DemoSpec.module)>>)
+.
+Proof.
+  eexists (ModPair.mk _ _ _); s.
+  esplits; eauto. instantiate (1:=tt).
+  econs; ss; i.
+  destruct SIMSKENVLINK.
+  exploit demo_unreach_local_preservation. i. des.
+  eapply match_states_sim with (match_states := match_states_ext_demo); ss.
+  - apply unit_ord_wf.
+  - ss. eauto.
+  - i. ss.
+    inv INITTGT. inv SAFESRC. inv H. clarify.
+    inv SIMARGS. ss.
+    esplits; eauto.
+    + econs; eauto.
+    + instantiate (2:=tt).
+      destruct x, st_init_tgt. ss.
+      rewrite VS, VS0 in VALS. inv VALS. inv H4. inv H2; ss.
+      econs; ss; eauto.
+      rewrite MEMSRC, MEMTGT. eauto.
+  - i. ss. des. inv SAFESRC.
+    set (sm_init_tgt := mkstate (get_arg st_init_src) (SimMemExt.tgt sm_arg)).
+    exists sm_init_tgt.
+    esplits. econs; ss.
+    + inv SIMARGS. ss. rewrite VS in *. inv VALS. inv H2; inv H3. eauto.
+    + inv SIMARGS. ss.
+  - i. ss. inv MATCH; eauto.
+  - i. ss. inv FINALSRC. inv MATCH.
+    esplits; eauto.
+    + econs. ss.
+    + econs; eauto. ss. clarify.
+  - right. ii. des.
+    esplits.
+    + i. inv MATCH; ss.
+      unfold safe_modsem in H.
+      exploit H. eapply star_refl. ii. des; clarify.
+    + ii. inv STEPTGT; inv MATCH; ss.
+      Unshelve. ss. eapply bot4.
+Qed.
+
+Lemma demo_ext_top
+  :
+    exists mp,
+      (<<SIM: @ModPair.sim SimMemExt.SimMemExt SimMemExt.SimSymbExtends SoundTop.Top mp>>)
+      /\ (<<SRC: mp.(ModPair.src) = (DemoSpec.module)>>)
+      /\ (<<TGT: mp.(ModPair.tgt) = (DemoSpec.module)>>)
+.
+Proof.
+  eexists (ModPair.mk _ _ _); s.
+  esplits; eauto. instantiate (1:=tt).
+  econs; ss; i.
+  destruct SIMSKENVLINK.
+  eapply match_states_sim with (match_states := match_states_ext_demo); ss.
+  - apply unit_ord_wf.
+  - eapply SoundTop.sound_state_local_preservation.
+  - i. ss.
+    inv INITTGT. inv SAFESRC. inv H. clarify.
+    inv SIMARGS. ss.
+    esplits; eauto.
+    + econs; eauto.
+    + instantiate (2:=tt).
+      destruct x, st_init_tgt. ss.
+      rewrite VS, VS0 in VALS. inv VALS. inv H4. inv H2; ss.
+      econs; ss; eauto.
+      rewrite MEMSRC, MEMTGT. eauto.
+  - i. ss. des. inv SAFESRC.
+    set (sm_init_tgt := mkstate (get_arg st_init_src) (SimMemExt.tgt sm_arg)).
+    exists sm_init_tgt.
+    esplits. econs; ss.
+    + inv SIMARGS. ss. rewrite VS in *. inv VALS. inv H2; inv H3. eauto.
+    + inv SIMARGS. ss.
+  - i. ss. inv MATCH; eauto.
+  - i. ss. inv FINALSRC. inv MATCH.
+    esplits; eauto.
+    + econs. ss.
+    + econs; eauto. ss. clarify.
+  - right. ii. des.
+    esplits.
+    + i. inv MATCH; ss.
+      unfold safe_modsem in H.
+      exploit H. eapply star_refl. ii. des; clarify.
+    + ii. inv STEPTGT; inv MATCH; ss.
+      Unshelve. ss. eapply bot4.
+Qed.
+
+Lemma demo_inj_drop_bot
+      (WF: Sk.wf (DemoSpec.module))
+  :
+    exists mp,
+      (<<SIM: @ModPair.sim SimMemInjC.SimMemInj SimSymbDrop.SimSymbDrop SoundTop.Top mp>>)
+      /\ (<<SRC: mp.(ModPair.src) = (DemoSpec.module)>>)
+      /\ (<<TGT: mp.(ModPair.tgt) = (DemoSpec.module)>>)
+      /\ (<<SSBOT: mp.(ModPair.ss) = bot1>>)
+.
+Proof.
+  eexists (ModPair.mk _ _ _); s.
+  esplits; eauto.
+  econs; ss; i.
+  { econs; ss; i; clarify.
+    inv WF. auto. }
+  eapply match_states_sim with (match_states := match_states_demo); ss.
+  - apply unit_ord_wf.
+  - eapply SoundTop.sound_state_local_preservation.
+  - i. ss.
+    inv INITTGT. inv SAFESRC. inv H. clarify.
+    inv SIMARGS. ss.
+    esplits; eauto.
+    + econs; eauto.
+    + refl.
+    + destruct x, st_init_tgt. ss.
+      rewrite VS, VS0 in VALS. inv VALS. inv H4. inv H2; ss.
+      econs; ss; eauto.
+      rewrite MEMSRC, MEMTGT. ss.
+  - i. ss. des. inv SAFESRC.
+    set (sm_init_tgt := mkstate (get_arg st_init_src) (SimMemInj.tgt sm_arg)).
+    exists sm_init_tgt.
+    esplits. econs; ss.
+    + inv SIMARGS. ss. rewrite VS in *. inv VALS. inv H2; inv H3. eauto.
+    + inv SIMARGS. ss.
+  - i. ss. inv MATCH; eauto.
+  - i. ss. inv FINALSRC. inv MATCH; inv MATCHST.
+    esplits; eauto.
+    + econs. ss.
+    + econs; eauto; ss. clarify.
+    + refl.
+  - right. ii. des.
+    esplits.
+    + i. inv MATCH; ss.
+      unfold safe_modsem in H.
+      exploit H. eapply star_refl. ii. des; clarify.
+    + ii. inv STEPTGT; inv MATCH; ss.
+      Unshelve. ss. eapply bot4.
+Qed.
+
+Lemma demo_inj_drop
+      (WF: Sk.wf (DemoSpec.module))
+  :
+    exists mp,
+      (<<SIM: @ModPair.sim SimMemInjC.SimMemInj SimSymbDrop.SimSymbDrop SoundTop.Top mp>>)
+      /\ (<<SRC: mp.(ModPair.src) = (DemoSpec.module)>>)
+      /\ (<<TGT: mp.(ModPair.tgt) = (DemoSpec.module)>>)
+.
+Proof.
+  exploit demo_inj_drop_bot; eauto. i. des. eauto.
+Qed.
+
+Lemma demo_inj_id
+      (WF: Sk.wf (DemoSpec.module))
+  :
+    exists mp,
+      (<<SIM: @ModPair.sim SimMemInjC.SimMemInj SimMemInjC.SimSymbId SoundTop.Top mp>>)
+      /\ (<<SRC: mp.(ModPair.src) = (DemoSpec.module)>>)
+      /\ (<<TGT: mp.(ModPair.tgt) = (DemoSpec.module)>>)
+.
+Proof.
+  apply sim_inj_drop_bot_id. apply demo_inj_drop_bot; auto.
+Qed.
